Typed reqres data structures

src/lib/communication/DY.Lib.Communication.Printing.fst
@@ -10,13 +10,19 @@ open DY.Lib.Communication.RequestResponse
 
 #set-options "--fuel 0 --ifuel 1 --z3cliopt 'smt.qi.eager_threshold=100'"
 
-val com_message_to_string: (bytes -> option string) -> (bytes -> option string) -> bytes -> option string
-let com_message_to_string msg_to_string reqres_payload_to_string b =
+val com_message_to_string:
+  #reqres_type:Type -> {|parseable_serializeable bytes reqres_type|} -> 
+  (bytes -> option string) -> (reqres_type -> string) -> bytes ->
+  option string
+let com_message_to_string #reqres_type msg_to_string reqres_payload_to_string b =
   match b with
   | PkeEnc pk nonce msg -> (
     match parse com_message_t msg with
     | Some (SigMessage _) -> Some "Error: SigMessage cannot be inside a PkeEnc encryption"
-    | Some (RequestMessage {request; key}) -> reqres_payload_to_string request
+    | Some (RequestMessage {request; key}) -> (
+      let? request_parsed = parse reqres_type request in 
+      Some (reqres_payload_to_string request_parsed)
+    )
     | Some (ResponseMessage _) -> Some "Error: ResponseMessage cannot be inside a PkeEnc encryption"
     | None -> Some (option_to_string msg_to_string b)
   )
@@ -47,7 +53,10 @@ let com_message_to_string msg_to_string reqres_payload_to_string b =
     | Some (RequestMessage _) -> Some "Error: RequestMessage cannot be send in plaintext"
     | Some (ResponseMessage {nonce; ciphertext}) -> (
       match ciphertext with
-      | AeadEnc key nonce msg ad -> reqres_payload_to_string msg
+      | AeadEnc key nonce response ad -> (
+        let? response_parsed = parse reqres_type response in 
+        Some (reqres_payload_to_string response_parsed)
+      )
       | _ -> Some "Error: response_envelope does not contain an AEAD ciphertext"
     )
     | None -> Some (option_to_string msg_to_string b)
@@ -78,45 +87,59 @@ let com_core_event_to_string payload_to_string =
         sender receiver (option_to_string payload_to_string payload))
   )))
 
-val com_reqres_event_to_string: {|comm_layer_reqres_tag|} -> (bytes -> option string) -> (string & (bytes -> option string))
-let com_reqres_event_to_string #tag payload_to_string =
+val com_reqres_event_to_string:
+  {|comm_layer_reqres_tag|} ->
+  #reqres_type:Type -> {|parseable_serializeable bytes reqres_type|} ->
+  (reqres_type -> string) -> 
+  (string & (bytes -> option string))
+let com_reqres_event_to_string #tag #reqres_type payload_to_string =
   (event_communication_reqres_event.tag, (fun b -> (
     let? cre = parse communication_reqres_event b in
     match cre with
-    | CommClientSendRequest client server request key -> 
+    | CommClientSendRequest client server request key -> (
+      let? request_parsed = parse reqres_type request in
       Some (Printf.sprintf "CommClientSendRequest client = %s, server = %s, request = (%s)"
-        client server (option_to_string payload_to_string request))
-    | CommServerReceiveRequest server request key -> 
+        client server (payload_to_string request_parsed))
+    )
+    | CommServerReceiveRequest server request key -> (
+      let? request_parsed = parse reqres_type request in
       Some (Printf.sprintf "CommServerReceiveRequest server = %s, request = (%s), key = %s"
-        server (option_to_string payload_to_string request) (bytes_to_string key))
-    | CommServerSendResponse server request response -> 
+        server (payload_to_string request_parsed) (bytes_to_string key))
+    )
+    | CommServerSendResponse server request response -> (
+      let? request_parsed = parse reqres_type request in
+      let? response_parsed = parse reqres_type response in
       Some (Printf.sprintf "CommServerSendResponse server = %s, request = %s, response = (%s)"
-        server (option_to_string payload_to_string request) (option_to_string payload_to_string response))
-    | CommClientReceiveResponse client server response key -> 
+        server (payload_to_string request_parsed) (payload_to_string response_parsed))
+    )
+    | CommClientReceiveResponse client server response key -> (
+      let? response_parsed = parse reqres_type response in
       Some (Printf.sprintf "CommClientReceiveResponse client = %s, server = %s, response = (%s), key = %s" 
-        client server (option_to_string payload_to_string response) (bytes_to_string key))
+        client server (payload_to_string response_parsed) (bytes_to_string key))
+    )
   )))
 
 val com_event_to_string:
   {|comm_layer_reqres_tag|} ->
-  (bytes -> option string) -> (bytes -> option string) ->
+  #reqres_type:Type -> {|parseable_serializeable bytes reqres_type|} ->
+  (bytes -> option string) -> (reqres_type -> string) ->
   list (string & (bytes -> option string))
-let com_event_to_string #tag core_payload_to_string reqres_payload_to_string =
+let com_event_to_string #tag #reqres_type core_payload_to_string reqres_payload_to_string =
   [com_core_event_to_string core_payload_to_string;
-    com_reqres_event_to_string reqres_payload_to_string]
+    com_reqres_event_to_string #tag #reqres_type reqres_payload_to_string]
 
-val com_state_to_string: (bytes -> option string) -> (string & (bytes -> option string))
-let com_state_to_string payload_to_string =
-  (local_state_communication_layer_session.tag, (fun b -> (
-    let? cs = parse communication_states b in
+val com_state_to_string: {|t:comm_layer_reqres_tag|} -> (#a:Type0) -> {|comparse_parser_serializer a|} -> (a -> string) -> (string & (bytes -> option string))
+let com_state_to_string #tag #a #ps payload_to_string =
+  ((local_state_communication_layer_session a).tag, (fun b -> (
+    let? cs = parse (communication_states a) b in
     match cs with
     | ClientSendRequest {server; request; key} -> 
       Some (Printf.sprintf "ClientSendRequest server = %s, payload = (%s), key = %s" 
-        server (option_to_string payload_to_string request) (bytes_to_string key))
+        server (payload_to_string request) (bytes_to_string key))
     | ServerReceiveRequest {request; key} -> 
       Some (Printf.sprintf "ServerReceiveRequest payload = (%s), key = %s"
-        (option_to_string payload_to_string request) (bytes_to_string key)) 
+        (payload_to_string request) (bytes_to_string key)) 
     | ClientReceiveResponse {server; response; key} -> 
       Some (Printf.sprintf "ClientReceiveResponse server = %s, payload = (%s), key = %s"
-        server (option_to_string payload_to_string response) (bytes_to_string key))
+        server (payload_to_string response) (bytes_to_string key))
   )))
