src/lib/communication/DY.Lib.Communication.RequestResponse.Lemmas.fst
@@ -21,20 +21,25 @@ open DY.Lib.Communication.RequestResponse.Invariants
 
 (*** Lemmas ***)
 
-val get_response_label: tr:trace -> comm_meta_data -> label
-let get_response_label tr req_meta_data = get_label #default_crypto_usages tr req_meta_data.key
+val get_response_label: tr:trace -> a:Type -> {|comparse_parser_serializer a|} -> comm_meta_data a -> label
+let get_response_label tr a #ps req_meta_data = get_label #default_crypto_usages tr req_meta_data.key
 
 val is_comm_response_payload:
   {|crypto_invariants|} ->
-  #a:Type -> {| parseable_serializeable bytes a |} ->
-  trace -> principal -> comm_meta_data -> a -> prop
-let is_comm_response_payload #cusg #a tr server req_meta_data payload =
-  is_well_formed a (is_knowable_by (get_response_label tr req_meta_data) tr) payload
+  #a:Type -> {|comparse_parser_serializer a|} ->
+  trace -> principal -> comm_meta_data a -> a -> prop
+let is_comm_response_payload #cusg #a #ps tr server req_meta_data payload =
+  is_well_formed a #ps_able (is_knowable_by (get_response_label tr a req_meta_data) tr) payload
 
-val comm_meta_data_knowable: {|crypto_invariants|} -> trace -> principal -> comm_meta_data -> prop
-let comm_meta_data_knowable #cinvs tr prin req_meta_data =
+val comm_meta_data_knowable: 
+  {|crypto_invariants|} ->
+  trace ->
+  a:Type -> {|comparse_parser_serializer a|} ->
+  principal -> comm_meta_data a ->
+  prop
+let comm_meta_data_knowable #cinvs tr a #ps prin req_meta_data =
   is_knowable_by (principal_label prin) tr req_meta_data.key /\
-  is_knowable_by (principal_label prin) tr req_meta_data.request
+  is_well_formed a #ps_able (is_knowable_by (principal_label prin) tr) req_meta_data.request
 
 /// The communication layer makes use of many lemmas with SMT patterns.
 /// These lemmas depend, however, on the communication layer predicates
@@ -60,12 +65,12 @@ let enable_reqres_comm_layer_lemmas preds =
   normalize_term_spec (reqres_comm_layer_lemmas_enabled preds)
 
 val send_request_proof:
-  {|comm_layer_reqres_tag|} ->
+  {|tag:comm_layer_reqres_tag|} ->
   {|protocol_invariants|} ->
-  #a:Type -> {| parseable_serializeable bytes a |} ->
+  #a:Type -> {|comparse_parser_serializer a|} ->
   tr:trace ->
   comm_keys_ids:communication_keys_sess_ids ->
-  higher_layer_preds:comm_reqres_higher_layer_event_preds a ->
+  higher_layer_preds:comm_reqres_higher_layer_event_preds a #ps_able ->
   client:principal -> server:principal -> request:a ->
   Lemma
   (requires
@@ -73,41 +78,41 @@ val send_request_proof:
     has_pki_invariant /\
     has_communication_layer_crypto_predicates /\
     has_communication_layer_reqres_event_predicates request_response_event_preconditions higher_layer_preds /\
-    has_communication_layer_state_predicates /\
+    has_communication_layer_state_predicates a /\
     higher_layer_preds.send_request tr client server request (comm_label client server) /\
-    is_well_formed a (is_knowable_by (comm_label client server) tr) request
+    is_well_formed a #ps_able (is_knowable_by (comm_label client server) tr) request
   )
   (ensures (
     match send_request comm_keys_ids client server request tr with
     | (None, tr_out) -> trace_invariant tr_out
     | (Some (_, cmeta_data), tr_out) -> (
       trace_invariant tr_out /\
-      comm_meta_data_knowable tr_out client cmeta_data
+      comm_meta_data_knowable tr_out a client cmeta_data
     )
   ))
   [SMTPat (trace_invariant tr);
   SMTPat (reqres_comm_layer_lemmas_enabled higher_layer_preds);
   SMTPat (send_request comm_keys_ids client server request tr)]
-let send_request_proof #tag #invs #a tr comm_keys_ids higher_layer_preds client server request =
-  reveal_opaque (`%send_request) (send_request #tag #a);
+let send_request_proof #tag #invs #a #ps tr comm_keys_ids higher_layer_preds client server request =
+  reveal_opaque (`%send_request) (send_request #tag #a #ps);
   enable_core_comm_layer_lemmas request_response_event_preconditions;
-  let request_bytes = serialize #bytes a request in
+  let request_bytes = serialize #bytes a #ps_able request in
   match send_request comm_keys_ids client server request tr with
   | (None, tr_out) -> (
     let (key, tr') = mk_rand (AeadKey comm_layer_aead_tag empty) (comm_label client server) 32 tr in
     let (sid, tr') = new_session_id client tr' in
-    let ((), tr') = set_state client sid (ClientSendRequest {server; request=request_bytes; key} <: communication_states) tr' in
+    let ((), tr') = set_state client sid (ClientSendRequest {server; request=request; key} <: communication_states a) tr' in
     higher_layer_preds.send_request_later tr tr' client server request (get_label tr' key);
     ()
   )
   | (Some _, tr_out) -> (
     let (key, tr') = mk_rand (AeadKey comm_layer_aead_tag empty) (comm_label client server) 32 tr in
     let (sid, tr') = new_session_id client tr' in
-    let ((), tr') = set_state client sid (ClientSendRequest {server; request=request_bytes; key} <: communication_states) tr' in
+    let ((), tr') = set_state client sid (ClientSendRequest {server; request; key} <: communication_states a) tr' in
     higher_layer_preds.send_request_later tr tr' client server request (get_label tr' key);
     let ((), tr') = trigger_event client (CommClientSendRequest client server request_bytes key) tr' in
     assert(trace_invariant tr');
-    let req_payload:com_message_t = RequestMessage {request=(serialize a request); key} in
+    let req_payload:com_message_t = RequestMessage {request=request_bytes; key} in
     let req_payload_bytes = serialize #bytes com_message_t req_payload in
     let (Some msg_id, tr') = send_confidential comm_keys_ids client server req_payload tr' in
 
@@ -121,10 +126,10 @@ let send_request_proof #tag #invs #a tr comm_keys_ids higher_layer_preds client 
 val receive_request_proof:
   {|tag:comm_layer_reqres_tag|} ->
   {|protocol_invariants|} ->
-  #a:Type -> {| parseable_serializeable bytes a |} ->
+  #a:Type -> {|ps:comparse_parser_serializer a|} ->
   tr:trace ->
   comm_keys_ids:communication_keys_sess_ids ->
-  higher_layer_preds:comm_reqres_higher_layer_event_preds a ->
+  higher_layer_preds:comm_reqres_higher_layer_event_preds a #ps_able ->
   server:principal -> msg_id:timestamp ->
   Lemma
   (requires
@@ -133,31 +138,32 @@ val receive_request_proof:
     has_pki_invariant /\
     has_communication_layer_reqres_crypto_predicates /\
     has_communication_layer_reqres_event_predicates request_response_event_preconditions higher_layer_preds /\
-    has_communication_layer_state_predicates
+    has_communication_layer_state_predicates a
   )
   (ensures (
     match receive_request comm_keys_ids server msg_id tr with
     | (None, tr_out) -> trace_invariant tr_out
     | (Some (payload, req_meta_data), tr_out) -> (
-      let payload_bytes = serialize a payload in
+      let payload_bytes = serialize a #ps_able payload in
       trace_invariant tr_out /\
       event_triggered tr_out server (CommServerReceiveRequest server payload_bytes req_meta_data.key) /\
-      is_well_formed a (is_knowable_by (principal_label server) tr_out) payload /\
-      is_well_formed a (is_knowable_by (get_response_label tr_out req_meta_data) tr_out) payload /\
-      payload_bytes == req_meta_data.request
+      is_well_formed a #ps_able (is_knowable_by (principal_label server) tr_out) payload /\
+      is_well_formed a #ps_able (is_knowable_by (get_response_label tr_out a req_meta_data) tr_out) payload /\
+      payload == req_meta_data.request
     )
   ))
   [SMTPat (trace_invariant tr);
   SMTPat (reqres_comm_layer_lemmas_enabled higher_layer_preds);
-  SMTPat (receive_request #tag #a comm_keys_ids server msg_id tr)]
-let receive_request_proof #tag #invs #a tr comm_keys_ids higher_layer_preds server msg_id =
-  reveal_opaque (`%receive_request) (receive_request #tag #a);
+  SMTPat (receive_request #tag #a #ps comm_keys_ids server msg_id tr)]
+let receive_request_proof #tag #invs #a #ps tr comm_keys_ids higher_layer_preds server msg_id =
+  reveal_opaque (`%receive_request) (receive_request #tag #a #ps);
   enable_core_comm_layer_lemmas request_response_event_preconditions;
-  match receive_request #tag #a comm_keys_ids server msg_id tr with
+  match receive_request comm_keys_ids server msg_id tr with
   | (None, tr_out) -> ()
   | (Some (payload, req_meta_data), tr_out) -> (
     let (Some req_msg_t, tr') = receive_confidential comm_keys_ids server msg_id tr in
     let RequestMessage req_msg = req_msg_t in
+    let Some request = parse a #ps_able req_msg.request in
 
     let req_msg_bytes = serialize com_message_t req_msg_t in
     let req_send_event client = CommClientSendRequest client server req_msg.request req_msg.key in
@@ -169,7 +175,7 @@ let receive_request_proof #tag #invs #a tr comm_keys_ids higher_layer_preds serv
     eliminate (exists client. event_triggered tr' client (req_send_event client)) \/
               (is_publishable tr' req_msg.request /\ is_publishable tr' req_msg.key)
     returns (
-      is_knowable_by (get_response_label tr' req_meta_data) tr' req_msg.request /\
+      is_knowable_by (get_response_label tr' a req_meta_data) tr' req_msg.request /\
       req_msg.key `has_usage tr'` (AeadKey comm_layer_aead_tag empty)
     )
     with _. eliminate exists client. event_triggered tr' client (req_send_event client)
@@ -182,12 +188,12 @@ let receive_request_proof #tag #invs #a tr comm_keys_ids higher_layer_preds serv
     and _. has_usage_publishable tr' req_msg.key (AeadKey comm_layer_aead_tag empty);
 
     // Relating knowledge of the request to knowledge of its fields
-    serialize_parse_inv_lemma #bytes a req_msg.request;
+    serialize_parse_inv_lemma #bytes a #ps_able req_msg.request;
     assert(is_comm_response_payload tr' server req_meta_data payload);
 
     let ((), tr') = trigger_event server (CommServerReceiveRequest server req_msg.request req_msg.key) tr' in
     let (sid', tr') = new_session_id server tr' in
-    let ((), tr') = set_state server sid' (ServerReceiveRequest {request=req_msg.request; key=req_msg.key} <: communication_states) tr' in
+    let ((), tr') = set_state server sid' (ServerReceiveRequest {request; key=req_msg.key} <: communication_states a) tr' in
     assert(tr' == tr_out);
     assert(trace_invariant tr_out);
     ()
@@ -197,13 +203,14 @@ let receive_request_proof #tag #invs #a tr comm_keys_ids higher_layer_preds serv
 
 val mk_comm_layer_response_nonce_proof:
   {|comm_layer_reqres_tag|} ->
+  #a:Type -> {|comparse_parser_serializer a|} ->
   {|protocol_invariants|} ->
   tr:trace ->
-  req_meta_data:comm_meta_data -> usg:usage ->
+  req_meta_data:comm_meta_data a -> usg:usage ->
   Lemma
   (requires
     trace_invariant tr /\
-    has_communication_layer_state_predicates /\
+    has_communication_layer_state_predicates a /\
     has_communication_layer_reqres_crypto_predicates /\
     bytes_well_formed tr req_meta_data.key
   )
@@ -211,36 +218,36 @@ val mk_comm_layer_response_nonce_proof:
     match mk_comm_layer_response_nonce req_meta_data usg tr with
     | (None, tr_out) -> trace_invariant tr_out
     | (Some nonce, tr_out) -> (
-      is_knowable_by (get_response_label tr_out req_meta_data) tr_out nonce
+      is_knowable_by (get_response_label tr_out a req_meta_data) tr_out nonce
     )
   ))
-let mk_comm_layer_response_nonce_proof #tag #invs tr req_meta_data usg =
-  reveal_opaque (`%mk_comm_layer_response_nonce) (mk_comm_layer_response_nonce)
+let mk_comm_layer_response_nonce_proof #tag #a #ps #invs tr req_meta_data usg =
+  reveal_opaque (`%mk_comm_layer_response_nonce) (mk_comm_layer_response_nonce #a)
 
 
 val compute_response_message_proof:
   {|comm_layer_reqres_tag|} ->
   {|crypto_invariants|} ->
-  #a:Type -> {| parseable_serializeable bytes a |} ->
+  #a:Type -> {|comparse_parser_serializer a|} ->
   tr:trace ->
   server:principal ->
-  key:bytes -> nonce:bytes -> request:bytes -> response:a ->
+  key:bytes -> nonce:bytes -> request:a -> response:a ->
   Lemma
   (requires
     has_communication_layer_reqres_crypto_predicates /\
     is_knowable_by (principal_label server) tr key /\
-    is_well_formed a (is_knowable_by (get_label tr key) tr) response /\
+    is_well_formed a #ps_able (is_knowable_by (get_label tr key) tr) response /\
     is_publishable tr nonce /\
     key `has_usage tr` (AeadKey comm_layer_aead_tag empty) /\
-    event_triggered tr server (CommServerSendResponse server request (serialize a response))
+    event_triggered tr server (CommServerSendResponse server (serialize a #ps_able request) (serialize a #ps_able response))
   )
   (ensures
     is_publishable tr (compute_response_message #a server key nonce response)
   )
-let compute_response_message_proof #tag #cinvs #a tr server key nonce request response =
+let compute_response_message_proof #tag #cinvs #a #ps tr server key nonce request response =
   reveal_opaque (`%compute_response_message) (compute_response_message #a);
-  let res_bytes = serialize a response in
-  serialize_wf_lemma a (is_knowable_by (get_label tr key) tr) response;
+  let res_bytes = serialize a #ps_able response in
+  serialize_wf_lemma a #ps_able (is_knowable_by (get_label tr key) tr) response;
   let ad:authenticated_data = {server} in
   let ad_bytes = serialize authenticated_data ad in
   serialize_wf_lemma authenticated_data (is_publishable tr) ad;
@@ -253,20 +260,18 @@ let compute_response_message_proof #tag #cinvs #a tr server key nonce request re
 val send_response_proof:
   {|comm_layer_reqres_tag|} ->
   {|protocol_invariants|} ->
-  #a:Type -> {| parseable_serializeable bytes a |} ->
+  #a:eqtype -> {|comparse_parser_serializer a|} ->
   tr:trace ->
-  higher_layer_preds:comm_reqres_higher_layer_event_preds a ->
-  server:principal -> req_meta_data:comm_meta_data -> response:a ->
+  higher_layer_preds:comm_reqres_higher_layer_event_preds a #ps_able ->
+  server:principal -> req_meta_data:comm_meta_data a -> response:a ->
   Lemma
   (requires
     trace_invariant tr /\
     has_communication_layer_reqres_crypto_predicates /\
     has_communication_layer_reqres_event_predicates request_response_event_preconditions higher_layer_preds /\
-    (match parse a req_meta_data.request with
-    | None -> False
-    | Some request -> higher_layer_preds.send_response tr server request response) /\
-    has_communication_layer_state_predicates /\
-    is_well_formed a (is_knowable_by (get_response_label tr req_meta_data) tr) response
+    higher_layer_preds.send_response tr server req_meta_data.request response /\
+    has_communication_layer_state_predicates a /\
+    is_well_formed a #ps_able (is_knowable_by (get_response_label tr a req_meta_data) tr) response
   )
   (ensures (
     let (_, tr_out) = send_response server req_meta_data response tr in
@@ -275,14 +280,14 @@ val send_response_proof:
   [SMTPat (trace_invariant tr);
   SMTPat (reqres_comm_layer_lemmas_enabled higher_layer_preds);
   SMTPat (send_response server req_meta_data response tr)]
-let send_response_proof #tag #invs #a tr higher_layer_preds server req_meta_data response =
-  reveal_opaque (`%send_response) (send_response #tag #a);
+let send_response_proof #tag #invs #a #ps tr higher_layer_preds server req_meta_data response =
+  reveal_opaque (`%send_response) (send_response #tag #a #ps);
   match send_response server req_meta_data response tr with
   | (None, tr_out) -> ()
   | (Some msg_id, tr_out) -> (
-    let (Some state, tr') = get_state server req_meta_data.sid tr in
+    let (Some state, tr'):(option (communication_states a) & trace) = get_state server req_meta_data.sid tr in
     let ServerReceiveRequest srr = state in
-    let ((), tr') = trigger_event server (CommServerSendResponse server req_meta_data.request (serialize a response)) tr' in
+    let ((), tr') = trigger_event server (CommServerSendResponse server (serialize a #ps_able req_meta_data.request) (serialize a #ps_able response)) tr' in
     let (nonce, tr') = mk_rand NoUsage public 32 tr' in
     compute_response_message_proof tr' server req_meta_data.key nonce req_meta_data.request response;
     let resp_msg_bytes = compute_response_message server req_meta_data.key nonce response in
@@ -297,7 +302,7 @@ let send_response_proof #tag #invs #a tr higher_layer_preds server req_meta_data
 val decode_response_proof:
   {|comm_layer_reqres_tag|} ->
   {|crypto_invariants|} ->
-  #a:Type -> {| parseable_serializeable bytes a |} ->
+  #a:Type -> {|comparse_parser_serializer a|} ->
   tr:trace ->
   client:principal -> server:principal ->
   key:bytes -> response:bytes ->
@@ -312,9 +317,9 @@ val decode_response_proof:
     match decode_response_message server key response with
     | None -> True
     | Some payload -> (
-      is_well_formed a (is_knowable_by (get_label tr key) tr) payload /\
-      is_knowable_by (get_label tr key) tr (serialize a payload) /\
-      (exists request. event_triggered tr server (CommServerSendResponse server request (serialize a payload))
+      is_well_formed a #ps_able (is_knowable_by (get_label tr key) tr) payload /\
+      is_knowable_by (get_label tr key) tr (serialize a #ps_able payload) /\
+      (exists request. event_triggered tr server (CommServerSendResponse server request (serialize a #ps_able payload))
         \/ is_corrupt tr (principal_label client) \/ is_corrupt tr (principal_label server))
     )
   ))
@@ -328,7 +333,7 @@ let decode_response_proof #tag #cinvs #a #ps tr client server key msg_bytes =
     serialize_wf_lemma authenticated_data (is_publishable tr) {server};
     let ad_bytes = serialize authenticated_data {server} in
     let Some res_bytes = aead_dec key nonce ciphertext ad_bytes in
-    serialize_parse_inv_lemma #bytes a #ps res_bytes;
+    serialize_parse_inv_lemma #bytes a #ps_able res_bytes;
     ()
   )
 #pop-options
@@ -336,44 +341,44 @@ let decode_response_proof #tag #cinvs #a #ps tr client server key msg_bytes =
 val receive_response_proof:
   {|tag:comm_layer_reqres_tag|} ->
   {|protocol_invariants|} ->
-  #a:Type -> {| parseable_serializeable bytes a |} ->
+  #a:Type -> {|comparse_parser_serializer a|} ->
   tr:trace ->
-  higher_layer_preds:comm_reqres_higher_layer_event_preds a ->
-  client:principal -> req_meta_data:comm_meta_data -> msg_id:timestamp ->
+  higher_layer_preds:comm_reqres_higher_layer_event_preds a #ps_able ->
+  client:principal -> req_meta_data:comm_meta_data a -> msg_id:timestamp ->
   Lemma
   (requires
     trace_invariant tr /\
     has_communication_layer_reqres_crypto_predicates /\
     has_communication_layer_reqres_event_predicates request_response_event_preconditions higher_layer_preds /\
-    has_communication_layer_state_predicates
+    has_communication_layer_state_predicates a
   )
   (ensures (
     match receive_response client req_meta_data msg_id tr with
     | (None, tr_out) -> trace_invariant tr_out
     | (Some (payload, _), tr_out) -> (
       trace_invariant tr_out /\
-      event_triggered tr_out client (CommClientReceiveResponse client req_meta_data.server (serialize a payload) req_meta_data.key) /\
-      is_well_formed a (is_knowable_by (get_label tr_out req_meta_data.key) tr_out) payload
+      event_triggered tr_out client (CommClientReceiveResponse client req_meta_data.server (serialize a #ps_able payload) req_meta_data.key) /\
+      is_well_formed a #ps_able (is_knowable_by (get_label tr_out req_meta_data.key) tr_out) payload
     )
   ))
   [SMTPat (trace_invariant tr);
   SMTPat (reqres_comm_layer_lemmas_enabled higher_layer_preds);
-  SMTPat (receive_response #tag #a client req_meta_data msg_id tr)]
-let receive_response_proof #tag #invs #a tr higher_layer_preds client req_meta_data msg_id =
-  reveal_opaque (`%receive_response) (receive_response #tag #a);
-  match receive_response #tag #a client req_meta_data msg_id tr with
+  SMTPat (receive_response client req_meta_data msg_id tr)]
+let receive_response_proof #tag #invs #a #ps tr higher_layer_preds client req_meta_data msg_id =
+  reveal_opaque (`%receive_response) (receive_response #tag #a #ps);
+  match receive_response #tag #a #ps client req_meta_data msg_id tr with
   | (None, tr_out) -> ()
   | (Some (response, _), tr_out) -> (
     let server = req_meta_data.server in
     let key = req_meta_data.key in
-    let (Some state, tr') = get_state client req_meta_data.sid tr in
+    let (Some state, tr'):(option (communication_states a) & trace) = get_state client req_meta_data.sid tr in
     let ClientSendRequest csr = state in
     let (Some resp_msg_bytes, tr') = recv_msg msg_id tr' in
     decode_response_proof #tag #invs.crypto_invs #a tr' client csr.server csr.key resp_msg_bytes;
     let Some response = decode_response_message csr.server csr.key resp_msg_bytes in
-    let ((), tr') = set_state client req_meta_data.sid (ClientReceiveResponse {server=csr.server; response=(serialize a response); key=csr.key} <: communication_states) tr' in
-    let ((), tr') = trigger_event client (CommClientReceiveResponse client csr.server (serialize a response) csr.key) tr' in
-    assert(event_triggered tr' client (CommClientReceiveResponse client csr.server (serialize a response) csr.key));
+    let ((), tr') = set_state client req_meta_data.sid (ClientReceiveResponse {server=csr.server; response; key=csr.key} <: communication_states a) tr' in
+    let ((), tr') = trigger_event client (CommClientReceiveResponse client csr.server (serialize a #ps_able response) csr.key) tr' in
+    assert(event_triggered tr' client (CommClientReceiveResponse client csr.server (serialize a #ps_able response) csr.key));
     assert(tr_out == tr');
     assert(trace_invariant tr_out);
     ()
