src/lib/communication/DY.Lib.Communication.RequestResponse.fst
@@ -6,18 +6,53 @@ open DY.Lib.State.PKI
 open DY.Lib.State.PrivateKeys
 open DY.Lib.Event.Typed
 open DY.Lib.State.Typed
+open DY.Lib.Comparse.Glue
 
 open DY.Lib.Communication.Data
 open DY.Lib.Communication.Core
 
 #set-options "--fuel 0 --ifuel 0 --z3cliopt 'smt.qi.eager_threshold=100'"
 
+(*** Layer Setup ***)
+
+class comparse_parser_serializer (a:Type) = {
+  ps_a: parser_serializer bytes a;
+  ps_able: parseable_serializeable bytes a;
+  [@@@FStar.Tactics.Typeclasses.no_method]
+  eq_property: squash (ps_able == mk_parseable_serializeable ps_a);
+}
+
+class comm_layer_reqres_tag = {
+  tag: string;
+}
+
+instance comm_layer_tag_core_reqres: comm_layer_core_tag = {
+  tag = "DY.Lib.Communication.Event.RequestResponse.Core"
+}
+
+val comm_layer_aead_tag: {|comm_layer_reqres_tag|} -> string
+let comm_layer_aead_tag #tag = tag.tag ^ ".Aead.Key"
+
+[@@with_bytes bytes]
+type comm_meta_data (a:Type) {|ps:comparse_parser_serializer a|} = {
+  key:bytes;
+  server:principal;
+  sid:state_id;
+  [@@@ with_parser #bytes ps.ps_a]
+  request:a;
+}
+
+%splice [ps_comm_meta_data] (gen_parser (`comm_meta_data))
+%splice [ps_comm_meta_data_is_well_formed] (gen_is_well_formed_lemma (`comm_meta_data))
+
+
 (*** States ***)
 
 [@@with_bytes bytes]
-type client_send_request = {
+type client_send_request (a:Type) {|ps:comparse_parser_serializer a|} = {
   server:principal;
-  request:bytes;
+  [@@@ with_parser #bytes ps.ps_a]
+  request:a;
   key:bytes
 }
 
@@ -25,8 +60,9 @@ type client_send_request = {
 %splice [ps_client_send_request_is_well_formed] (gen_is_well_formed_lemma (`client_send_request))
 
 [@@with_bytes bytes]
-type server_receive_request = {
-  request:bytes;
+type server_receive_request (a:Type) {|ps:comparse_parser_serializer a|} = {
+  [@@@ with_parser #bytes ps.ps_a]
+  request:a;
   key:bytes
 }
 
@@ -34,9 +70,10 @@ type server_receive_request = {
 %splice [ps_server_receive_request_is_well_formed] (gen_is_well_formed_lemma (`server_receive_request))
 
 [@@with_bytes bytes]
-type client_receive_response = {
+type client_receive_response (a:Type) {|ps:comparse_parser_serializer a|} = {
   server:principal;
-  response:bytes;
+  [@@@ with_parser #bytes ps.ps_a]
+  response:a;
   key:bytes
 }
 
@@ -44,22 +81,22 @@ type client_receive_response = {
 %splice [ps_client_receive_response_is_well_formed] (gen_is_well_formed_lemma (`client_receive_response))
 
 [@@with_bytes bytes]
-type communication_states =
-  | ClientSendRequest: client_send_request -> communication_states
-  | ServerReceiveRequest: server_receive_request -> communication_states
-  | ClientReceiveResponse: client_receive_response -> communication_states
+type communication_states (a:Type) {|ps:comparse_parser_serializer a|} =
+  | ClientSendRequest: client_send_request a -> communication_states a
+  | ServerReceiveRequest: server_receive_request a -> communication_states a
+  | ClientReceiveResponse: client_receive_response a -> communication_states a
 
 #push-options "--ifuel 1"
 %splice [ps_communication_states] (gen_parser (`communication_states))
 %splice [ps_communication_states_is_well_formed] (gen_is_well_formed_lemma (`communication_states))
 #pop-options
 
-instance parseable_serializeable_bytes_communication_states: parseable_serializeable bytes communication_states
-  = mk_parseable_serializeable ps_communication_states
+instance parseable_serializeable_bytes_communication_states (a:Type) {|comparse_parser_serializer a|}: parseable_serializeable bytes (communication_states a)
+  = mk_parseable_serializeable (ps_communication_states a)
 
-instance local_state_communication_layer_session: local_state communication_states = {
-  tag = "DY.Lib.Communication.State.RequestResponse";
-  format = parseable_serializeable_bytes_communication_states;
+instance local_state_communication_layer_session {|t:comm_layer_reqres_tag|} (a:Type) {|comparse_parser_serializer a|}: local_state (communication_states a) = {
+  tag = t.tag ^ ".State";
+  format = parseable_serializeable_bytes_communication_states a;
 }
 
 [@@with_bytes bytes]
@@ -74,34 +111,10 @@ type communication_reqres_event =
 %splice [ps_communication_reqres_event_is_well_formed] (gen_is_well_formed_lemma (`communication_reqres_event))
 #pop-options
 
-class comm_layer_reqres_tag = {
-  tag: string;
-}
-
 instance event_communication_reqres_event {|t:comm_layer_reqres_tag|}: event communication_reqres_event = {
-  tag = t.tag;
+  tag = t.tag ^ ".Event";
   format = mk_parseable_serializeable ps_communication_reqres_event;
 }
-
-instance comm_layer_tag_core_reqres: comm_layer_core_tag = {
-  tag = "DY.Lib.Communication.Event.RequestResponse.Core"
-}
-
-(*** Layer Setup ***)
-
-val comm_layer_aead_tag: {|comm_layer_reqres_tag|} -> string
-let comm_layer_aead_tag #tag = tag.tag ^ ".Aead.Key"
-
-[@@with_bytes bytes]
-type comm_meta_data = {
-  key:bytes;
-  server:principal;
-  sid:state_id;
-  request:bytes;
-}
-
-%splice [ps_comm_meta_data] (gen_parser (`comm_meta_data))
-%splice [ps_comm_meta_data_is_well_formed] (gen_is_well_formed_lemma (`comm_meta_data))
 
 
 (*** API ***)
@@ -109,49 +122,49 @@ type comm_meta_data = {
 [@@ "opaque_to_smt"]
 val send_request:
   {|comm_layer_reqres_tag|} ->
-  #a:Type -> {| parseable_serializeable bytes a |} ->
+  #a:Type -> {|comparse_parser_serializer a|} ->
   communication_keys_sess_ids ->
   principal -> principal -> a ->
-  traceful (option (timestamp & comm_meta_data))
-let send_request #tag #a comm_keys_ids client server request =
+  traceful (option (timestamp & comm_meta_data a))
+let send_request #tag #a #ps comm_keys_ids client server request =
   let* key = mk_rand (AeadKey comm_layer_aead_tag empty) (comm_label client server) 32 in
-  let payload_bytes = serialize #bytes a request in
+  let payload_bytes:bytes = serialize a #ps_able request in
   let* sid = new_session_id client in
-  set_state client sid (ClientSendRequest {server; request=payload_bytes; key} <: communication_states);*
+  set_state client sid (ClientSendRequest {server; request; key} <: communication_states a);*
   trigger_event client (CommClientSendRequest client server payload_bytes key);*
   let req_payload:com_message_t = RequestMessage {request=payload_bytes; key} in
   let*? msg_id = send_confidential comm_keys_ids client server req_payload in
-  let req_meta_data = {key; server; sid; request=payload_bytes} in
+  let req_meta_data:comm_meta_data a = {key; server; sid; request} in
   return (Some (msg_id, req_meta_data))
 
 [@@ "opaque_to_smt"]
 val receive_request:
   {|comm_layer_reqres_tag|} ->
-  #a:Type -> {| parseable_serializeable bytes a |} ->
+  #a:Type -> {|comparse_parser_serializer a|} ->
   communication_keys_sess_ids ->
   principal -> timestamp ->
-  traceful (option (a & comm_meta_data))
-let receive_request #tag #a comm_keys_ids server msg_id =
+  traceful (option (a & comm_meta_data a))
+let receive_request #tag #a #ps comm_keys_ids server msg_id =
   let*? req_msg_t:com_message_t = receive_confidential comm_keys_ids server msg_id in
   guard_tr (RequestMessage? req_msg_t);*?
   let RequestMessage req_msg = req_msg_t in
-  let*? request = return (parse a req_msg.request) in
+  let*? request = return (parse a #ps_able req_msg.request) in
   trigger_event server (CommServerReceiveRequest server req_msg.request req_msg.key);*
   let* sid = new_session_id server in
-  set_state server sid (ServerReceiveRequest {request=req_msg.request; key=req_msg.key} <: communication_states);*
-  let req_meta_data = {key=req_msg.key; server; sid; request=req_msg.request} in
+  set_state server sid (ServerReceiveRequest {request; key=req_msg.key} <: communication_states a);*
+  let req_meta_data:comm_meta_data a = {key=req_msg.key; server; sid; request} in
   return (Some (request, req_meta_data))
 
 [@@ "opaque_to_smt"]
-val mk_comm_layer_response_nonce: comm_meta_data -> usage -> traceful (option bytes)
-let mk_comm_layer_response_nonce req_meta_data usg =
+val mk_comm_layer_response_nonce: #a:Type -> {|comparse_parser_serializer a|} -> comm_meta_data a -> usage -> traceful (option bytes)
+let mk_comm_layer_response_nonce #a #ps_a req_meta_data usg =
   let* tr = get_trace in
   let* nonce = mk_rand usg (get_label #default_crypto_usages tr req_meta_data.key) 32 in
   return (Some nonce)
 
 [@@ "opaque_to_smt"]
-val mk_comm_layer_response_nonce_labeled: comm_meta_data -> usage -> label -> traceful (option bytes)
-let mk_comm_layer_response_nonce_labeled req_meta_data usg lab =
+val mk_comm_layer_response_nonce_labeled: #a:Type -> {|comparse_parser_serializer a|} -> comm_meta_data a -> usage -> label -> traceful (option bytes)
+let mk_comm_layer_response_nonce_labeled #a #ps_a req_meta_data usg lab =
   let* tr = get_trace in
   let lab_join = join lab (get_label #default_crypto_usages tr req_meta_data.key) in
   let* nonce = mk_rand usg lab_join 32 in
@@ -159,10 +172,10 @@ let mk_comm_layer_response_nonce_labeled req_meta_data usg lab =
 
 [@@ "opaque_to_smt"]
 val compute_response_message:
-  #a:Type -> {| parseable_serializeable bytes a |} ->
+  #a:Type -> {|comparse_parser_serializer a|} ->
   principal -> bytes -> bytes -> a -> bytes
-let compute_response_message #a server key nonce response =
-  let res_bytes = serialize a response in
+let compute_response_message #a #ps server key nonce response =
+  let res_bytes = serialize a #ps_able response in
   let ad:authenticated_data = {server} in
   let ad_bytes = serialize authenticated_data ad in
   let ciphertext = aead_enc key nonce res_bytes ad_bytes in
@@ -171,15 +184,15 @@ let compute_response_message #a server key nonce response =
 [@@ "opaque_to_smt"]
 val send_response:
   {|comm_layer_reqres_tag|} ->
-  #a:Type -> {| parseable_serializeable bytes a |} ->
-  principal -> comm_meta_data -> a -> traceful (option timestamp)
-let send_response #tag #a server req_meta_data response =
+  #a:eqtype -> {|comparse_parser_serializer a|} ->
+  principal -> comm_meta_data a -> a -> traceful (option timestamp)
+let send_response #tag #a #ps server req_meta_data response =
   let*? state = get_state server req_meta_data.sid in
   guard_tr (ServerReceiveRequest? state);*?
   let ServerReceiveRequest srr = state in
   guard_tr (srr.key = req_meta_data.key);*?
   guard_tr (srr.request = req_meta_data.request);*?
-  trigger_event server (CommServerSendResponse server srr.request (serialize a response));*
+  trigger_event server (CommServerSendResponse server (serialize a #ps_able srr.request) (serialize a #ps_able response));*
   let* nonce = mk_rand NoUsage public 32 in
   let resp_msg = compute_response_message server req_meta_data.key nonce response in
   let* msg_id = send_msg resp_msg in
@@ -188,32 +201,32 @@ let send_response #tag #a server req_meta_data response =
 [@@ "opaque_to_smt"]
 val decode_response_message:
   {|comm_layer_reqres_tag|} ->
-  #a:Type -> {| parseable_serializeable bytes a |} ->
+  #a:Type -> {|comparse_parser_serializer a|} ->
   principal -> bytes -> bytes -> option a
-let decode_response_message #tag #a server key msg_bytes =
+let decode_response_message #tag #a #ps server key msg_bytes =
   let? resp_env_t:com_message_t = parse com_message_t msg_bytes in
   guard (ResponseMessage? resp_env_t);?
   let ResponseMessage resp_env = resp_env_t in
   let ad:authenticated_data = {server} in
   let ad_bytes = serialize authenticated_data ad in
   let? resp_bytes = aead_dec key resp_env.nonce resp_env.ciphertext ad_bytes in
-  let? resp = parse a resp_bytes in
+  let? resp = parse a #ps_able resp_bytes in
   Some resp
 
 [@@ "opaque_to_smt"]
 val receive_response:
   {|comm_layer_reqres_tag|} ->
-  #a:Type -> {| parseable_serializeable bytes a |} ->
-  principal -> comm_meta_data -> timestamp ->
-  traceful (option (a & comm_meta_data))
-let receive_response #tag #a client req_meta_data msg_id =
-  let*? state = get_state client req_meta_data.sid in
+  #a:Type -> {|comparse_parser_serializer a|} ->
+  principal -> comm_meta_data a -> timestamp ->
+  traceful (option (a & comm_meta_data a))
+let receive_response #tag #a #ps client req_meta_data msg_id =
+  let*? state:communication_states a = get_state client req_meta_data.sid in
   guard_tr (ClientSendRequest? state);*?
   let ClientSendRequest csr = state in
   let*? resp_msg_bytes = recv_msg msg_id in
   let*? payload = return (decode_response_message csr.server csr.key resp_msg_bytes) in
   guard_tr (csr.server = req_meta_data.server);*?
   guard_tr (csr.key = req_meta_data.key);*?
-  set_state client req_meta_data.sid (ClientReceiveResponse {server=csr.server; response=(serialize a payload); key=csr.key} <: communication_states);*
-  trigger_event client (CommClientReceiveResponse client csr.server (serialize a payload) csr.key);*
+  set_state client req_meta_data.sid (ClientReceiveResponse {server=csr.server; response=payload; key=csr.key} <: communication_states a);*
+  trigger_event client (CommClientReceiveResponse client csr.server (serialize a #ps_able payload) csr.key);*
   return (Some (payload, req_meta_data))
